spec/Correctness_WOTS.ec
@@ -1,3 +1,4 @@
 (*
-
+    We first prove that the equivalence between the extracted EC and the preprocessed EC
+    We then prove that the preprocessed EC is equivalent to the specification (so the extracted EC is also equivalent to the spec)
 *)
