spec/extraction/XMSS_IMPL_PP.ec
@@ -27,13 +27,13 @@ module Mp(SC:Syscall_t) = {
     return (out);
   }
 
-  proc __ull_to_bytes_32 (out:W8.t Array32.t, in_0:W64.t) : W8.t Array32.t = {
+  proc __ull_to_bytes_2 (out:W8.t Array2.t, in_0:W64.t) : W8.t Array2.t = {
     var aux: int;
 
     var i:int;
 
     aux <- (- 1);
-    i <- (32 - 1);
+    i <- (2 - 1);
     while (aux < i) {
       out.[i] <- (truncateu8 in_0);
       in_0 <- (in_0 `>>` (W8.of_int 8));
@@ -57,13 +57,13 @@ module Mp(SC:Syscall_t) = {
     return (out);
   }
 
-  proc __ull_to_bytes_2 (out:W8.t Array2.t, in_0:W64.t) : W8.t Array2.t = {
+  proc __ull_to_bytes_32 (out:W8.t Array32.t, in_0:W64.t) : W8.t Array32.t = {
     var aux: int;
 
     var i:int;
 
     aux <- (- 1);
-    i <- (2 - 1);
+    i <- (32 - 1);
     while (aux < i) {
       out.[i] <- (truncateu8 in_0);
       in_0 <- (in_0 `>>` (W8.of_int 8));
@@ -196,19 +196,6 @@ module Mp(SC:Syscall_t) = {
     return (a);
   }
 
-  proc __memset_u8_4 (a:W8.t Array4.t, value:W8.t) : W8.t Array4.t = {
-
-    var i:W64.t;
-
-    i <- (W64.of_int 0);
-
-    while ((i \ult (W64.of_int 4))) {
-      a.[(W64.to_uint i)] <- value;
-      i <- (i + (W64.of_int 1));
-    }
-    return (a);
-  }
-
   proc __memset_u8_128 (a:W8.t Array128.t, value:W8.t) : W8.t Array128.t = {
 
     var i:W64.t;
@@ -216,6 +203,19 @@ module Mp(SC:Syscall_t) = {
     i <- (W64.of_int 0);
 
     while ((i \ult (W64.of_int 128))) {
+      a.[(W64.to_uint i)] <- value;
+      i <- (i + (W64.of_int 1));
+    }
+    return (a);
+  }
+
+  proc __memset_u8_4 (a:W8.t Array4.t, value:W8.t) : W8.t Array4.t = {
+
+    var i:W64.t;
+
+    i <- (W64.of_int 0);
+
+    while ((i \ult (W64.of_int 4))) {
       a.[(W64.to_uint i)] <- value;
       i <- (i + (W64.of_int 1));
     }
@@ -237,21 +237,6 @@ module Mp(SC:Syscall_t) = {
       i <- (i + (W64.of_int 1));
     }
     return ();
-  }
-
-  proc __memcpy_u8u8_128_32 (out:W8.t Array128.t, offset:W64.t,
-                             in_0:W8.t Array32.t) : W8.t Array128.t * W64.t = {
-
-    var i:W64.t;
-
-    i <- (W64.of_int 0);
-
-    while ((i \ult (W64.of_int 32))) {
-      out.[(W64.to_uint offset)] <- in_0.[(W64.to_uint i)];
-      i <- (i + (W64.of_int 1));
-      offset <- (offset + (W64.of_int 1));
-    }
-    return (out, offset);
   }
 
   proc __memcpy_u8u8_128_64 (out:W8.t Array128.t, offset:W64.t,
@@ -284,8 +269,8 @@ module Mp(SC:Syscall_t) = {
     return (out, offset);
   }
 
-  proc __memcpy_u8u8_64_32 (out:W8.t Array64.t, offset:W64.t,
-                            in_0:W8.t Array32.t) : W8.t Array64.t * W64.t = {
+  proc __memcpy_u8u8_128_32 (out:W8.t Array128.t, offset:W64.t,
+                             in_0:W8.t Array32.t) : W8.t Array128.t * W64.t = {
 
     var i:W64.t;
 
@@ -329,8 +314,8 @@ module Mp(SC:Syscall_t) = {
     return (out, offset);
   }
 
-  proc __memcpy_u8u8_2144_32 (out:W8.t Array2144.t, offset:W64.t,
-                              in_0:W8.t Array32.t) : W8.t Array2144.t * W64.t = {
+  proc __memcpy_u8u8_64_32 (out:W8.t Array64.t, offset:W64.t,
+                            in_0:W8.t Array32.t) : W8.t Array64.t * W64.t = {
 
     var i:W64.t;
 
@@ -344,10 +329,18 @@ module Mp(SC:Syscall_t) = {
     return (out, offset);
   }
 
-  proc _memcpy_u8u8_128_32 (out:W8.t Array128.t, offset:W64.t,
-                            in_0:W8.t Array32.t) : W8.t Array128.t * W64.t = {
+  proc __memcpy_u8u8_2144_32 (out:W8.t Array2144.t, offset:W64.t,
+                              in_0:W8.t Array32.t) : W8.t Array2144.t * W64.t = {
 
-    (out, offset) <@ __memcpy_u8u8_128_32 (out, offset, in_0);
+    var i:W64.t;
+
+    i <- (W64.of_int 0);
+
+    while ((i \ult (W64.of_int 32))) {
+      out.[(W64.to_uint offset)] <- in_0.[(W64.to_uint i)];
+      i <- (i + (W64.of_int 1));
+      offset <- (offset + (W64.of_int 1));
+    }
     return (out, offset);
   }
 
@@ -365,10 +358,10 @@ module Mp(SC:Syscall_t) = {
     return (out, offset);
   }
 
-  proc _memcpy_u8u8_64_32 (out:W8.t Array64.t, offset:W64.t,
-                           in_0:W8.t Array32.t) : W8.t Array64.t * W64.t = {
+  proc _memcpy_u8u8_128_32 (out:W8.t Array128.t, offset:W64.t,
+                            in_0:W8.t Array32.t) : W8.t Array128.t * W64.t = {
 
-    (out, offset) <@ __memcpy_u8u8_64_32 (out, offset, in_0);
+    (out, offset) <@ __memcpy_u8u8_128_32 (out, offset, in_0);
     return (out, offset);
   }
 
@@ -386,15 +379,10 @@ module Mp(SC:Syscall_t) = {
     return (out, offset);
   }
 
-  proc _x_memcpy_u8u8_128_32 (out:W8.t Array128.t, offset:W64.t,
-                              in_0:W8.t Array32.t) : W8.t Array128.t * W64.t = {
+  proc _memcpy_u8u8_64_32 (out:W8.t Array64.t, offset:W64.t,
+                           in_0:W8.t Array32.t) : W8.t Array64.t * W64.t = {
 
-    out <- out;
-    offset <- offset;
-    in_0 <- in_0;
-    (out, offset) <@ _memcpy_u8u8_128_32 (out, offset, in_0);
-    out <- out;
-    offset <- offset;
+    (out, offset) <@ __memcpy_u8u8_64_32 (out, offset, in_0);
     return (out, offset);
   }
 
@@ -422,13 +410,13 @@ module Mp(SC:Syscall_t) = {
     return (out, offset);
   }
 
-  proc _x_memcpy_u8u8_64_32 (out:W8.t Array64.t, offset:W64.t,
-                             in_0:W8.t Array32.t) : W8.t Array64.t * W64.t = {
+  proc _x_memcpy_u8u8_128_32 (out:W8.t Array128.t, offset:W64.t,
+                              in_0:W8.t Array32.t) : W8.t Array128.t * W64.t = {
 
     out <- out;
     offset <- offset;
     in_0 <- in_0;
-    (out, offset) <@ _memcpy_u8u8_64_32 (out, offset, in_0);
+    (out, offset) <@ _memcpy_u8u8_128_32 (out, offset, in_0);
     out <- out;
     offset <- offset;
     return (out, offset);
@@ -453,6 +441,18 @@ module Mp(SC:Syscall_t) = {
     offset <- offset;
     in_0 <- in_0;
     (out, offset) <@ _memcpy_u8u8_96_32 (out, offset, in_0);
+    out <- out;
+    offset <- offset;
+    return (out, offset);
+  }
+
+  proc _x_memcpy_u8u8_64_32 (out:W8.t Array64.t, offset:W64.t,
+                             in_0:W8.t Array32.t) : W8.t Array64.t * W64.t = {
+
+    out <- out;
+    offset <- offset;
+    in_0 <- in_0;
+    (out, offset) <@ _memcpy_u8u8_64_32 (out, offset, in_0);
     out <- out;
     offset <- offset;
     return (out, offset);
@@ -528,9 +528,9 @@ module Mp(SC:Syscall_t) = {
     return (out, offset);
   }
 
-  proc __memcpy_u8u8_2_32_2144 (out:W8.t Array32.t, out_offset:W64.t,
+  proc __memcpy_u8u8_2_64_2144 (out:W8.t Array64.t, out_offset:W64.t,
                                 in_0:W8.t Array2144.t, in_offset:W64.t,
-                                bytes:W64.t) : W8.t Array32.t * W64.t * W64.t = {
+                                bytes:W64.t) : W8.t Array64.t * W64.t * W64.t = {
 
     var i:W64.t;
 
@@ -545,9 +545,9 @@ module Mp(SC:Syscall_t) = {
     return (out, out_offset, in_offset);
   }
 
-  proc __memcpy_u8u8_2_64_2144 (out:W8.t Array64.t, out_offset:W64.t,
+  proc __memcpy_u8u8_2_32_2144 (out:W8.t Array32.t, out_offset:W64.t,
                                 in_0:W8.t Array2144.t, in_offset:W64.t,
-                                bytes:W64.t) : W8.t Array64.t * W64.t * W64.t = {
+                                bytes:W64.t) : W8.t Array32.t * W64.t * W64.t = {
 
     var i:W64.t;
 
@@ -604,22 +604,6 @@ module Mp(SC:Syscall_t) = {
     return (out_ptr, out_offset, in_offset);
   }
 
-  proc __memcpy_u8pu8_32 (out:W64.t, offset:W64.t, in_0:W8.t Array32.t) : 
-  W64.t * W64.t = {
-
-    var i:W64.t;
-
-    i <- (W64.of_int 0);
-
-    while ((i \ult (W64.of_int 32))) {
-      Glob.mem <-
-      storeW8 Glob.mem (W64.to_uint (out + offset)) (in_0.[(W64.to_uint i)]);
-      offset <- (offset + (W64.of_int 1));
-      i <- (i + (W64.of_int 1));
-    }
-    return (out, offset);
-  }
-
   proc __memcpy_u8pu8_4 (out:W64.t, offset:W64.t, in_0:W8.t Array4.t) : 
   W64.t * W64.t = {
 
@@ -636,10 +620,19 @@ module Mp(SC:Syscall_t) = {
     return (out, offset);
   }
 
-  proc _memcpy_u8pu8_32 (out:W64.t, offset:W64.t, in_0:W8.t Array32.t) : 
+  proc __memcpy_u8pu8_32 (out:W64.t, offset:W64.t, in_0:W8.t Array32.t) : 
   W64.t * W64.t = {
 
-    (out, offset) <@ __memcpy_u8pu8_32 (out, offset, in_0);
+    var i:W64.t;
+
+    i <- (W64.of_int 0);
+
+    while ((i \ult (W64.of_int 32))) {
+      Glob.mem <-
+      storeW8 Glob.mem (W64.to_uint (out + offset)) (in_0.[(W64.to_uint i)]);
+      offset <- (offset + (W64.of_int 1));
+      i <- (i + (W64.of_int 1));
+    }
     return (out, offset);
   }
 
@@ -650,15 +643,10 @@ module Mp(SC:Syscall_t) = {
     return (out, offset);
   }
 
-  proc _x_memcpy_u8pu8_32 (out:W64.t, offset:W64.t, in_0:W8.t Array32.t) : 
+  proc _memcpy_u8pu8_32 (out:W64.t, offset:W64.t, in_0:W8.t Array32.t) : 
   W64.t * W64.t = {
 
-    out <- out;
-    offset <- offset;
-    in_0 <- in_0;
-    (out, offset) <@ _memcpy_u8pu8_32 (out, offset, in_0);
-    out <- out;
-    offset <- offset;
+    (out, offset) <@ __memcpy_u8pu8_32 (out, offset, in_0);
     return (out, offset);
   }
 
@@ -669,6 +657,18 @@ module Mp(SC:Syscall_t) = {
     offset <- offset;
     in_0 <- in_0;
     (out, offset) <@ _memcpy_u8pu8_4 (out, offset, in_0);
+    out <- out;
+    offset <- offset;
+    return (out, offset);
+  }
+
+  proc _x_memcpy_u8pu8_32 (out:W64.t, offset:W64.t, in_0:W8.t Array32.t) : 
+  W64.t * W64.t = {
+
+    out <- out;
+    offset <- offset;
+    in_0 <- in_0;
+    (out, offset) <@ _memcpy_u8pu8_32 (out, offset, in_0);
     out <- out;
     offset <- offset;
     return (out, offset);
@@ -1204,6 +1204,43 @@ module Mp(SC:Syscall_t) = {
     return (out, addr);
   }
 
+  proc __base_w_3_2 (output:W32.t Array3.t, input:W8.t Array2.t) : W32.t Array3.t = {
+
+    var in_0:W64.t;
+    var out:W64.t;
+    var bits:W64.t;
+    var consumed:W64.t;
+    var total:W8.t;
+    var total_32:W32.t;
+    var _of_:bool;
+    var _cf_:bool;
+    var _sf_:bool;
+    var _zf_:bool;
+    var  _0:bool;
+
+    in_0 <- (W64.of_int 0);
+    out <- (W64.of_int 0);
+    bits <- (W64.of_int 0);
+    consumed <- (W64.of_int 0);
+
+    while ((consumed \ult (W64.of_int 3))) {
+      if ((bits = (W64.of_int 0))) {
+        total <- input.[(W64.to_uint in_0)];
+        in_0 <- (in_0 + (W64.of_int 1));
+        bits <- (bits + (W64.of_int 8));
+      } 
+      bits <- (bits - (W64.of_int 4));
+      total_32 <- (zeroextu32 total);
+      (_of_, _cf_, _sf_,  _0, _zf_, total_32) <- SHR_32 total_32
+      (truncateu8 bits);
+      total_32 <- (total_32 `&` (W32.of_int (16 - 1)));
+      output.[(W64.to_uint out)] <- total_32;
+      out <- (out + (W64.of_int 1));
+      consumed <- (consumed + (W64.of_int 1));
+    }
+    return (output);
+  }
+
   proc __base_w_67_32 (output:W32.t Array67.t, input:W8.t Array32.t) : 
   W32.t Array67.t = {
 
@@ -1225,43 +1262,6 @@ module Mp(SC:Syscall_t) = {
     consumed <- (W64.of_int 0);
 
     while ((consumed \ult (W64.of_int 67))) {
-      if ((bits = (W64.of_int 0))) {
-        total <- input.[(W64.to_uint in_0)];
-        in_0 <- (in_0 + (W64.of_int 1));
-        bits <- (bits + (W64.of_int 8));
-      } 
-      bits <- (bits - (W64.of_int 4));
-      total_32 <- (zeroextu32 total);
-      (_of_, _cf_, _sf_,  _0, _zf_, total_32) <- SHR_32 total_32
-      (truncateu8 bits);
-      total_32 <- (total_32 `&` (W32.of_int (16 - 1)));
-      output.[(W64.to_uint out)] <- total_32;
-      out <- (out + (W64.of_int 1));
-      consumed <- (consumed + (W64.of_int 1));
-    }
-    return (output);
-  }
-
-  proc __base_w_3_2 (output:W32.t Array3.t, input:W8.t Array2.t) : W32.t Array3.t = {
-
-    var in_0:W64.t;
-    var out:W64.t;
-    var bits:W64.t;
-    var consumed:W64.t;
-    var total:W8.t;
-    var total_32:W32.t;
-    var _of_:bool;
-    var _cf_:bool;
-    var _sf_:bool;
-    var _zf_:bool;
-    var  _0:bool;
-
-    in_0 <- (W64.of_int 0);
-    out <- (W64.of_int 0);
-    bits <- (W64.of_int 0);
-    consumed <- (W64.of_int 0);
-
-    while ((consumed \ult (W64.of_int 3))) {
       if ((bits = (W64.of_int 0))) {
         total <- input.[(W64.to_uint in_0)];
         in_0 <- (in_0 + (W64.of_int 1));
